Start updating the proofs in BottomUp

src/Transforms/BottomUp.dfy
@@ -17,7 +17,7 @@ module Bootstrap.Transforms.BottomUp {
   import opened Generic
   import Shallow
 
-  predicate MapChildrenPreservesPre(f: Expr --> Expr, post: Expr -> bool)
+  predicate {:verify false} MapChildrenPreservesPre(f: Expr --> Expr, post: Expr -> bool)
   // This predicate gives us the conditions for which, if we deeply apply `f` to all
   // the children of an expression, then the resulting expression satisfies the pre
   // of `f` (i.e., we can call `f` on it).
@@ -36,7 +36,7 @@ module Bootstrap.Transforms.BottomUp {
        ==> f.requires(e')
   }
 
-  predicate TransformerMatchesPrePost(f: Expr --> Expr, post: Expr -> bool)
+  predicate {:verify false} TransformerMatchesPrePost(f: Expr --> Expr, post: Expr -> bool)
   // This predicate gives us the conditions for which, if we deeply apply `f` to an
   // expression, the resulting expression satisfies the postcondition we give for `f`.
   //
@@ -51,13 +51,13 @@ module Bootstrap.Transforms.BottomUp {
   }
 
   // FIXME(CPC) move?
-  predicate TransformerShallowPreservesRel(f: Expr --> Expr, rel: (Expr, Expr) -> bool)
+  predicate {:verify false} TransformerShallowPreservesRel(f: Expr --> Expr, rel: (Expr, Expr) -> bool)
   // `f` relates its input and its output with `rel`.
   {
     forall e | f.requires(e) :: rel(e, f(e))
   }
 
-  predicate TransformerDeepPreservesRel(f: Expr --> Expr, rel: (Expr, Expr) -> bool)
+  predicate {:verify false} TransformerDeepPreservesRel(f: Expr --> Expr, rel: (Expr, Expr) -> bool)
   // This predicate is quite general, but is to be used in the following setting:
   // if we apply `f` on all the children of `e`, leading to an expression `e'`, then we
   // can relate `e` and `f(e')` with `rel`.
@@ -69,7 +69,7 @@ module Bootstrap.Transforms.BottomUp {
        ==> rel(e, f(e'))
   }
 
-  predicate IsBottomUpTransformer(f: Expr --> Expr, post: Expr -> bool, rel: (Expr,Expr) -> bool)
+  predicate {:verify false} IsBottomUpTransformer(f: Expr --> Expr, post: Expr -> bool, rel: (Expr,Expr) -> bool)
   // Predicate for ``BottomUpTransformer``
   {
     && TransformerMatchesPrePost(f, post)
@@ -79,23 +79,23 @@ module Bootstrap.Transforms.BottomUp {
 
   // Identity bottom-up transformer: we need it only because we need a witness when
   // defining ``BottomUpTransformer``, to prove that the type is inhabited.
-  const IdentityTransformer: ExprTransformer :=
+  const {:verify false} IdentityTransformer: ExprTransformer :=
     TR(d => d, _ => true, (_,_) => true)
 
-  lemma IdentityMatchesPrePost()
+  lemma {:verify false} IdentityMatchesPrePost()
     ensures TransformerMatchesPrePost(IdentityTransformer.f, IdentityTransformer.post)
   { }
 
-  lemma IdentityPreservesPre()
+  lemma {:verify false} IdentityPreservesPre()
     ensures MapChildrenPreservesPre(IdentityTransformer.f, IdentityTransformer.post)
   { }
 
-  lemma IdentityPreservesRel()
+  lemma {:verify false} IdentityPreservesRel()
     ensures TransformerDeepPreservesRel(IdentityTransformer.f, IdentityTransformer.rel)
   { }
 
   // FIXME(CPC): Move to equivs (use a datatype to make this a member function)
-  predicate RelCanBeMapLifted(rel: (Expr, Expr) -> bool)
+  predicate {:verify false} RelCanBeMapLifted(rel: (Expr, Expr) -> bool)
   // In many situations, the binary relation between the input and the output is transitive
   // and can be lifted through the map function.
   {
@@ -107,15 +107,15 @@ module Bootstrap.Transforms.BottomUp {
 
   // A bottom-up transformer, i.e.: a transformer we can recursively apply bottom-up to
   // an expression, and get the postcondition we expect on the resulting expression.
-  type BottomUpTransformer = tr: ExprTransformer | IsBottomUpTransformer(tr.f, tr.post, tr.rel)
+  type {:verify false} BottomUpTransformer = tr: ExprTransformer | IsBottomUpTransformer(tr.f, tr.post, tr.rel)
     witness (IdentityMatchesPrePost();
              IdentityPreservesPre();
              IdentityPreservesRel();
              IdentityTransformer)
 
-  predicate TODO() { false }
+  predicate {:verify false} TODO() { false }
 
-  function method MapChildren_Expr(e: Expr, tr: BottomUpTransformer) :
+  function method {:verify false} MapChildren_Expr(e: Expr, tr: BottomUpTransformer) :
     (e': Expr)
     decreases e, 0
     requires Deep.AllChildren_Expr(e, tr.f.requires)
@@ -143,7 +143,6 @@ module Bootstrap.Transforms.BottomUp {
         assert Exprs.ConstructorsMatch(e, e');
         e'
       case VarDecl(vdecls, ovals) =>
-        assume TODO();
         var ovals' :=
           match ovals
             case Some(vals) => Exprs.Some(Seq.Map(e requires e in vals => Map_Expr(e, tr), vals))
@@ -151,17 +150,9 @@ module Bootstrap.Transforms.BottomUp {
         var e' := Expr.VarDecl(vdecls, ovals');
         e'
       case Update(vars, vals) =>
-        assume TODO();
         var vals' := Seq.Map(e requires e in vals => Map_Expr(e, tr), vals);
         var e' := Expr.Update(vars, vals');
         e'
-/*          case Bind(vars, vals, body) =>
-        assume TODO();
-        var vals' := Seq.Map(e requires e in vals => Map_Expr(e, tr), vals);
-        Map_All_IsMap(e requires e in vals => Map_Expr(e, tr), vals);
-        var e' := Expr.Bind(vars, vals', Map_Expr(body, tr));
-        assert Exprs.ConstructorsMatch(e, e');
-        e'*/
       case If(cond, thn, els) =>
         var e' := Expr.If(Map_Expr(cond, tr), Map_Expr(thn, tr), Map_Expr(els, tr));
         assert Exprs.ConstructorsMatch(e, e');
@@ -170,7 +161,7 @@ module Bootstrap.Transforms.BottomUp {
   }
 
   // Apply a transformer bottom-up on an expression.
-  function method Map_Expr(e: Expr, tr: BottomUpTransformer) : (e': Expr)
+  function method {:verify false} Map_Expr(e: Expr, tr: BottomUpTransformer) : (e': Expr)
     decreases e, 1
     requires Deep.All_Expr(e, tr.f.requires)
     ensures Deep.All_Expr(e', tr.post)
@@ -179,7 +170,7 @@ module Bootstrap.Transforms.BottomUp {
     tr.f(MapChildren_Expr(e, tr))
   }
 
-  function method Map_Expr_Transformer'(tr: BottomUpTransformer) :
+  function method {:verify false} Map_Expr_Transformer'(tr: BottomUpTransformer) :
     (tr': Transformer_<Expr,Expr>)
   // We can write aggregated statements only in lemmas.
   // This forced me to cut this definition into pieces...
@@ -189,7 +180,7 @@ module Bootstrap.Transforms.BottomUp {
        tr.rel)
   }
 
-  lemma Map_Expr_Transformer'_Lem(tr: BottomUpTransformer)
+  lemma {:verify false} Map_Expr_Transformer'_Lem(tr: BottomUpTransformer)
     ensures Map_Expr_Transformer'(tr).HasValidRel()
   {
     var tr' := Map_Expr_Transformer'(tr);
@@ -219,7 +210,7 @@ module Bootstrap.Transforms.BottomUp {
     }
   }
 
-  function method Map_Expr_Transformer(tr: BottomUpTransformer) :
+  function method {:verify false} Map_Expr_Transformer(tr: BottomUpTransformer) :
     (tr': ExprTransformer)
   // Given a bottom-up transformer `tr`, return a transformer which applies `tr` in
   // a bottom-up manner.
@@ -229,7 +220,7 @@ module Bootstrap.Transforms.BottomUp {
     tr'
   }
 
-  function method {:opaque} Map_Method(m: Method, tr: BottomUpTransformer) :
+  function method {:verify false} {:opaque} Map_Method(m: Method, tr: BottomUpTransformer) :
     (m': Method)
     requires Deep.All_Method(m, tr.f.requires)
     ensures Deep.All_Method(m', tr.post)
@@ -239,7 +230,7 @@ module Bootstrap.Transforms.BottomUp {
     Shallow.Map_Method(m, Map_Expr_Transformer(tr))
   }
 
-  function method {:opaque} Map_Program(p: Program, tr: BottomUpTransformer) :
+  function method {:verify false} {:opaque} Map_Program(p: Program, tr: BottomUpTransformer) :
     (p': Program)
     requires Deep.All_Program(p, tr.f.requires)
     ensures Deep.All_Program(p', tr.post)
@@ -265,14 +256,14 @@ module Bootstrap.Transforms.Proofs.BottomUp_ {
   import opened Semantics.Equiv
 
 
-  type Expr = Syntax.Expr
-  type WV = Interp.Value // FIXME
-  type EqWV = Interp.EqWV // FIXME
-  type Context = Values.Context
+  type {:verify false} Expr = Syntax.Expr
+  type {:verify false} WV = Interp.Value // FIXME
+  type {:verify false} EqWV = Interp.EqWV // FIXME
+  type {:verify false} Context = Values.Context
 
   // TODO: maybe not necessary to make this opaque
   // FIXME(CPC): Change to Interp.Expr and remove SupportsInterp below
-  predicate {:opaque} EqInterp_CanBeMapLifted_Pre(e: Expr, e': Expr, env: Environment, ctx: State, ctx': State)
+  predicate {:verify false} {:opaque} EqInterp_CanBeMapLifted_Pre(e: Expr, e': Expr, env: Environment, ctx: State, ctx': State)
   {
     && EqState(ctx, ctx')
     && Exprs.ConstructorsMatch(e, e')
@@ -282,14 +273,14 @@ module Bootstrap.Transforms.Proofs.BottomUp_ {
   }
 
   // TODO: maybe not necessary to make this opaque
-  predicate {:opaque} EqInterp_CanBeMapLifted_Post(e: Expr, e': Expr, env: Environment, ctx: State, ctx': State)
+  predicate {:verify false} {:opaque} EqInterp_CanBeMapLifted_Post(e: Expr, e': Expr, env: Environment, ctx: State, ctx': State)
     requires EqInterp_CanBeMapLifted_Pre(e, e', env, ctx, ctx')
   {
     reveal EqInterp_CanBeMapLifted_Pre();
     EqInterpResultValue(InterpExpr(e, env, ctx), InterpExpr(e', env, ctx'))
   }
 
-  lemma EqInterp_Expr_CanBeMapLifted_Lem(e: Expr, e': Expr, env: Environment, ctx: State, ctx': State)
+  lemma {:verify false} EqInterp_Expr_CanBeMapLifted_Lem(e: Expr, e': Expr, env: Environment, ctx: State, ctx': State)
     requires EqInterp_CanBeMapLifted_Pre(e, e', env, ctx, ctx')
     ensures EqInterp_CanBeMapLifted_Post(e, e', env, ctx, ctx')
     decreases e, env, 1
@@ -325,10 +316,10 @@ module Bootstrap.Transforms.Proofs.BottomUp_ {
         EqInterp_Expr_If_CanBeMapLifted_Lem(e, e', env, ctx, ctx');
       }
       case VarDecl(_, _) => {
-        assume TODO();
+        EqInterp_Expr_VarDecl_CanBeMapLifted_Lem(e, e', env, ctx, ctx');
       }
       case Update(_, _) => {
-        assume TODO();
+        EqInterp_Expr_Update_CanBeMapLifted_Lem(e, e', env, ctx, ctx');
       }
       case _ => {
         // Unsupported branch
@@ -338,7 +329,7 @@ module Bootstrap.Transforms.Proofs.BottomUp_ {
     }
   }
 
-  lemma EqInterp_Expr_Var_CanBeMapLifted_Lem(e: Interp.Expr, e': Interp.Expr, env: Environment, ctx: State, ctx': State)
+  lemma {:verify false} EqInterp_Expr_Var_CanBeMapLifted_Lem(e: Interp.Expr, e': Interp.Expr, env: Environment, ctx: State, ctx': State)
     requires e.Var?
     requires e'.Var?
     requires EqInterp_CanBeMapLifted_Pre(e, e', env, ctx, ctx')
@@ -356,7 +347,7 @@ module Bootstrap.Transforms.Proofs.BottomUp_ {
   }
 
   // FIXME(CPC): Can this lemma and the following ones use Interp.Expr?
-  lemma EqInterp_Expr_Literal_CanBeMapLifted_Lem(e: Interp.Expr, e': Interp.Expr, env: Environment, ctx: State, ctx': State)
+  lemma {:verify false} EqInterp_Expr_Literal_CanBeMapLifted_Lem(e: Interp.Expr, e': Interp.Expr, env: Environment, ctx: State, ctx': State)
     requires e.Literal?
     requires e'.Literal?
     requires EqInterp_CanBeMapLifted_Pre(e, e', env, ctx, ctx')
@@ -370,7 +361,7 @@ module Bootstrap.Transforms.Proofs.BottomUp_ {
     reveal InterpLiteral();
   }
 
-  lemma EqInterp_Expr_Abs_CanBeMapLifted_Lem(e: Interp.Expr, e': Interp.Expr, env: Environment, ctx: State, ctx': State)
+  lemma {:verify false} EqInterp_Expr_Abs_CanBeMapLifted_Lem(e: Interp.Expr, e': Interp.Expr, env: Environment, ctx: State, ctx': State)
     requires e.Abs?
     requires e'.Abs?
     requires EqInterp_CanBeMapLifted_Pre(e, e', env, ctx, ctx')
@@ -407,7 +398,7 @@ module Bootstrap.Transforms.Proofs.BottomUp_ {
     }
   }
 
-  lemma EqInterp_Expr_AbsClosure_CanBeMapLifted_Lem(cv: WV, cv': WV, env: Environment, argvs: seq<WV>, argvs': seq<WV>)
+  lemma {:verify false} EqInterp_Expr_AbsClosure_CanBeMapLifted_Lem(cv: WV, cv': WV, env: Environment, argvs: seq<WV>, argvs': seq<WV>)
     requires cv.Closure?
     requires cv'.Closure?
     requires |argvs| == |argvs'| == |cv.vars|
@@ -433,7 +424,7 @@ module Bootstrap.Transforms.Proofs.BottomUp_ {
     }
   }
 
-  lemma EqInterp_Expr_ApplyLazy_CanBeMapLifted_Lem(e: Interp.Expr, e': Interp.Expr, env: Environment, ctx: State, ctx': State)
+  lemma {:verify false} EqInterp_Expr_ApplyLazy_CanBeMapLifted_Lem(e: Interp.Expr, e': Interp.Expr, env: Environment, ctx: State, ctx': State)
     requires e.Apply? && e.aop.Lazy?
     requires e'.Apply? && e'.aop.Lazy?
     requires EqInterp_CanBeMapLifted_Pre(e, e', env, ctx, ctx')
@@ -483,7 +474,7 @@ module Bootstrap.Transforms.Proofs.BottomUp_ {
     }
   }
 
-  lemma EqInterp_Expr_ApplyEager_CanBeMapLifted_Lem(e: Interp.Expr, e': Interp.Expr, env: Environment, ctx: State, ctx': State)
+  lemma {:verify false} EqInterp_Expr_ApplyEager_CanBeMapLifted_Lem(e: Interp.Expr, e': Interp.Expr, env: Environment, ctx: State, ctx': State)
     requires e.Apply? && e.aop.Eager?
     requires e'.Apply? && e'.aop.Eager?
     requires EqInterp_CanBeMapLifted_Pre(e, e', env, ctx, ctx')
@@ -559,7 +550,7 @@ module Bootstrap.Transforms.Proofs.BottomUp_ {
   }
 
   // TODO: e and e' should be the same actually
-  lemma EqInterp_Expr_UnaryOp_CanBeMapLifted_Lem(
+  lemma {:verify false} EqInterp_Expr_UnaryOp_CanBeMapLifted_Lem(
     e: Interp.Expr, e': Interp.Expr, op: UnaryOp, v: WV, v': WV
   )
     requires !op.MemberSelect?
@@ -618,7 +609,7 @@ module Bootstrap.Transforms.Proofs.BottomUp_ {
   // TODO: we could split this lemma, whose proof is big (though straightforward),
   // but it is a bit annoying to do...
   // TODO: e and e' should be the same actually
-  lemma EqInterp_Expr_BinaryOp_CanBeMapLifted_Lem(
+  lemma {:verify false} EqInterp_Expr_BinaryOp_CanBeMapLifted_Lem(
     e: Interp.Expr, e': Interp.Expr, bop: BinaryOp, v0: WV, v1: WV, v0': WV, v1': WV
   )
     requires !bop.BV? && !bop.Datatypes?
@@ -791,7 +782,7 @@ module Bootstrap.Transforms.Proofs.BottomUp_ {
   }
 
   // TODO: e and e' should be the same actually
-  lemma EqInterp_Expr_TernaryOp_CanBeMapLifted_Lem(
+  lemma {:verify false} EqInterp_Expr_TernaryOp_CanBeMapLifted_Lem(
     e: Interp.Expr, e': Interp.Expr, top: TernaryOp, v0: WV, v1: WV, v2: WV, v0': WV, v1': WV, v2': WV
   )
     requires EqValue(v0, v0')
@@ -815,7 +806,7 @@ module Bootstrap.Transforms.Proofs.BottomUp_ {
     }
   }
 
-  lemma EqInterp_Expr_Display_CanBeMapLifted_Lem(
+  lemma {:verify false} EqInterp_Expr_Display_CanBeMapLifted_Lem(
     e: Interp.Expr, e': Interp.Expr, kind: Types.CollectionKind, vs: seq<WV>, vs': seq<WV>
   )
     requires EqSeqValue(vs, vs')
@@ -853,7 +844,7 @@ module Bootstrap.Transforms.Proofs.BottomUp_ {
     }
   }
 
-  lemma EqInterp_Expr_FunctionCall_CanBeMapLifted_Lem(
+  lemma {:verify false} EqInterp_Expr_FunctionCall_CanBeMapLifted_Lem(
     e: Interp.Expr, e': Interp.Expr, env: Environment, f: WV, f': WV, argvs: seq<WV>, argvs': seq<WV>
   )
     requires EqValue(f, f')
@@ -898,7 +889,7 @@ module Bootstrap.Transforms.Proofs.BottomUp_ {
     }
   }
 
-  lemma EqInterp_Expr_If_CanBeMapLifted_Lem(e: Interp.Expr, e': Interp.Expr, env: Environment, ctx: State, ctx': State)
+  lemma {:verify false} EqInterp_Expr_If_CanBeMapLifted_Lem(e: Interp.Expr, e': Interp.Expr, env: Environment, ctx: State, ctx': State)
     requires e.If?
     requires e'.If?
     requires EqInterp_CanBeMapLifted_Pre(e, e', env, ctx, ctx')
@@ -949,7 +940,107 @@ module Bootstrap.Transforms.Proofs.BottomUp_ {
     }
   }
 
-  lemma EqInterp_CanBeMapLifted_Lem()
+  lemma {:verify false} EqInterp_Expr_VarDecl_CanBeMapLifted_Lem(e: Interp.Expr, e': Interp.Expr, env: Environment, ctx: State, ctx': State)
+    requires e.VarDecl?
+    requires e'.VarDecl?
+    requires EqInterp_CanBeMapLifted_Pre(e, e', env, ctx, ctx')
+    ensures EqInterp_CanBeMapLifted_Post(e, e', env, ctx, ctx')
+    decreases e, env, 0
+  {
+    assume TODO();
+  }
+
+  lemma {:verify true} EqInterp_Expr_Update_CanBeMapLifted_Lem(e: Interp.Expr, e': Interp.Expr, env: Environment, ctx: State, ctx': State)
+    requires e.Update?
+    requires e'.Update?
+    requires EqInterp_CanBeMapLifted_Pre(e, e', env, ctx, ctx')
+    ensures EqInterp_CanBeMapLifted_Post(e, e', env, ctx, ctx')
+    decreases e, env, 0
+  {      
+    reveal EqInterp_CanBeMapLifted_Pre();
+    reveal EqInterp_CanBeMapLifted_Post();
+
+    reveal InterpExpr();
+    reveal SupportsInterp();
+
+    var res := InterpExpr(e, env, ctx);
+    var res' := InterpExpr(e', env, ctx');
+
+    var Update(vars, vals) := e;
+    var Update(vars', vals') := e';
+
+    // The rhs evaluate to similar results
+    var res0 := InterpExprs(vals, env, ctx);
+    var res0' := InterpExprs(vals', env, ctx');
+    InterpExprs_EqInterp_Lem(vals, vals', env, ctx, ctx');
+    assert EqInterpResult(EqSeqValue, res0, res0');
+    
+    if res0.Success? {
+      // Dafny crashes if we try to deconstruct the `Return`s in the match.
+      // See: https://github.com/dafny-lang/dafny/issues/2258
+      var Return(valsvs, ctx0) := res0.value;
+      var Return(valsvs', ctx0') := res0'.value;
+
+      var ctx1 := ctx0.(locals := AugmentContext(ctx.locals, vars, valsvs));
+      var ctx1' := ctx0'.(locals := AugmentContext(ctx'.locals, vars, valsvs'));
+
+      // assert EqState(ctx1, ctx1');
+
+    // var Return(vals, ctx) :- InterpExprs(vals, env, ctx);
+    // var ctx := ctx.(locals := AugmentContext(ctx.locals, vars, vals));
+    // Success(Return(Unit, ctx))
+ 
+      assume TODO();
+    }
+    else {
+      // Trivial
+    }
+    
+/*      match (res0, res0') {
+      case (Success(res0), Success(res0')) => {
+        // Dafny crashes if we try to deconstruct the `Return`s in the match.
+        // See: https://github.com/dafny-lang/dafny/issues/2258
+        var Return(argvs, ctx0) := res0;
+        var Return(argvs', ctx0') := res0';
+ 
+        match (op, op') {
+          case (UnaryOp(op), UnaryOp(op')) => {
+            assert op == op';
+            EqInterp_Expr_UnaryOp_CanBeMapLifted_Lem(e, e', op, argvs[0], argvs'[0]);
+            assert EqInterpResultValue(res, res');
+          }
+          case (BinaryOp(bop), BinaryOp(bop')) => {
+            assert bop == bop';
+            EqInterp_Expr_BinaryOp_CanBeMapLifted_Lem(e, e', bop, argvs[0], argvs[1], argvs'[0], argvs'[1]);
+            assert EqInterpResultValue(res, res');
+          }
+          case (TernaryOp(top), TernaryOp(top')) => {
+            assert top == top';
+            EqInterp_Expr_TernaryOp_CanBeMapLifted_Lem(e, e', top, argvs[0], argvs[1], argvs[2], argvs'[0], argvs'[1], argvs'[2]);
+            assert EqInterpResultValue(res, res');
+          }
+          case (Builtin(Display(ty)), Builtin(Display(ty'))) => {
+            assert ty == ty';
+            EqInterp_Expr_Display_CanBeMapLifted_Lem(e, e', ty.kind, argvs, argvs');
+            assert EqInterpResultValue(res, res');
+          }
+          case (FunctionCall(), FunctionCall()) => {
+            EqInterp_Expr_FunctionCall_CanBeMapLifted_Lem(e, e', env, argvs[0], argvs'[0], argvs[1..], argvs'[1..]);
+            assert EqInterpResultValue(res, res');
+          }
+          case _ => {
+            // Impossible branch
+            assert false;
+          }
+        }
+      }
+      case (Failure(_), _) => {
+        // Trivial
+      }
+    } */
+  }
+
+  lemma {:verify false} EqInterp_CanBeMapLifted_Lem()
     ensures RelCanBeMapLifted(EqInterp)
   {
     forall e, e'
